TotalViperHelperML.thy
@@ -20,6 +20,9 @@ fun REPEAT_DETERM' tac x =
 fun apply_tacs_seq [] = K (all_tac)
  | apply_tacs_seq (tac :: tacs) = tac THEN' (apply_tacs_seq tacs)
 
+fun del_simps [] ctxt = ctxt
+ |  del_simps (thm::thms) ctxt = del_simps thms (Simplifier.del_simp thm ctxt)
+
 (* This basically applies the cut rule \<lbrakk>P; P \<Longrightarrow> Q\<rbrakk> \<Longrightarrow> Q. It has the same effect as
    cut_tac, except that one must first prove P (while in cut_tac one must first prove P \<Longrightarrow> Q) *)
 fun revcut_tac rule i = resolve0_tac [revcut_rl] i THEN resolve0_tac [rule] i
