ViperBoogieEndToEndML.thy
@@ -1,5 +1,5 @@
 theory ViperBoogieEndToEndML
-imports ViperBoogieEndToEnd CPGHelperML ViperBoogieHelperML
+imports ViperBoogieEndToEnd CPGHelperML ViperBoogieHelperML ViperBoogieFunctionInst
 begin
 
 ML \<open>
@@ -29,6 +29,117 @@ ML \<open>
          simplify_continuation ctxt) ctxt) THEN'
     (Rmsg' "Post Framing Init - Propagate 2" (resolve_tac ctxt @{thms stmt_rel_propagate_same_rel}) ctxt) THEN'
     (Rmsg' "Post Framing Init - Assume Good State" (progress_assume_good_state_rel_tac ctxt (#ctxt_wf_thm basic_info) (#tr_def_thm basic_info)) ctxt)
+
+\<close>
+
+lemmas axioms_sat_proof_del = vbpl_absval_ty.simps type_of_val.simps full_ext_env.simps
+
+method simplify_bound_var_tac = 
+   (simp add: inversion_type_of_vbpl_val_equalities realv_inversion_type_of_vbpl_val del: axioms_sat_proof_del id_apply),
+   (erule conjE, erule exE)+,
+   (simp only: id_apply)
+
+method axiom_proof_init =
+   (simp only: expr_sat_def),
+   ((rule RedForallT_True | rule RedForAllTrue)+ | succeed),
+   (simplify_bound_var_tac) ? \<comment>\<open>only makes sense of there is at least one universal value quantifier\<close>
+
+ML \<open>
+   
+  fun del_simps [] ctxt = ctxt
+   |  del_simps (thm::thms) ctxt = del_simps thms (Simplifier.del_simp thm ctxt)
+
+
+  type axiom_tac_data = {
+    lookup_const_tac : (int -> tactic),
+    finterp_eval_tac : (Proof.context -> term -> int -> tactic),
+    fun_interp_inst_def_thm: thm
+  }
+
+  val Rmsg' = run_and_print_if_fail_2_tac' 
+
+
+  fun extract_fun_enum_bpl t =
+    case t of 
+      @{term "Trueprop"} $ t' => extract_fun_enum_bpl t'
+    | Const (@{const_name HOL.eq}, _) $ lhs $ _ => extract_fun_enum_bpl lhs
+    | Const (@{const_name "fun_interp_vpr_bpl"}, _) 
+           $ _ (* program *)
+           $ _ (* type representation *)
+           $ _ (* field translation *)
+           $ fun_enum
+           $ _ (* type parameters *)
+           $ _ (* function arguments *) =>
+             fun_enum
+    | _ => raise TERM ("goal is not fun_interp_vpr_bpl", [t])
+
+  fun axiom_aux_tac ctxt lookup_const_thms del_thms (axiom_tac_data : axiom_tac_data) = 
+    FIRST_AND_THEN' [
+       resolve_tac ctxt @{thms RedVar},
+       resolve_tac ctxt @{thms RedBVar},
+       resolve_tac ctxt @{thms RedBinOp},
+
+       resolve_tac ctxt @{thms RedFunOp},
+       resolve_tac ctxt @{thms RedLit},
+       Rmsg' "Unexpected case" (K no_tac) ctxt
+    ] [
+      (* Var *)
+      (#lookup_const_tac axiom_tac_data |> SOLVED'), 
+      (* BVar *)
+       Rmsg' "RedBVar simp" (assm_full_simp_solved_tac ctxt) ctxt,
+      (* BinOp *)
+       (fn i => fn st => axiom_aux_tac ctxt lookup_const_thms del_thms axiom_tac_data i st) THEN'
+       (fn i => fn st => axiom_aux_tac ctxt lookup_const_thms del_thms axiom_tac_data i st) THEN'
+       Rmsg' "RedBinOp simp" (assm_full_simp_solved_tac ctxt) ctxt,
+      (* FunOp *)
+       (Rmsg' "RedFunOp init"
+         (simp_only_tac [#fun_interp_inst_def_thm axiom_tac_data] ctxt THEN'
+          resolve_tac ctxt @{thms fun_interp_vpr_bpl_concrete_lookup[OF fun_repr_concrete_inj]} THEN'
+          fast_tac (ctxt addIs @{thms fun_repr_concrete.simps})) ctxt) THEN'
+      
+       (* function arguments *)
+       (fn i => fn st => axiom_aux_list_tac ctxt lookup_const_thms del_thms axiom_tac_data i st) THEN'
+       (* function interpretation evaluation *)
+       (Rmsg' "RedFunOp finish"
+             (SUBGOAL (fn (t,i) => (#finterp_eval_tac axiom_tac_data) ctxt (extract_fun_enum_bpl (Logic.strip_assums_concl t)) i) 
+                                            |> SOLVED') ctxt),
+       (* Lit *)
+       K all_tac,
+       (* unexpected case *)
+       K no_tac
+     ]
+
+and axiom_aux_list_tac ctxt lookup_const_thms del_thms (axiom_tac_data : axiom_tac_data) =
+    FIRST_AND_THEN'
+      [ resolve_tac ctxt @{thms RedExpListCons},
+        resolve_tac ctxt @{thms RedExpListNil}
+      ] 
+      [ (* cons *)
+        ((fn i => fn st => axiom_aux_tac ctxt lookup_const_thms del_thms axiom_tac_data i st) |> SOLVED') THEN'
+        (fn i => fn st => axiom_aux_list_tac ctxt lookup_const_thms del_thms axiom_tac_data i st),
+        (* nil *)
+        K all_tac
+      ]
+
+fun finterp_eval_concrete_tac del_thms ctxt t = 
+  case t of
+    Const (@{const_name FReadHeap}, _) => 
+     asm_full_simp_tac (del_simps  (@{thm fun_upd_apply}::del_thms) (add_simps @{thms lift_fun_bpl_def heap_upd_ty_preserved_2_basic} ctxt))  THEN'
+     asm_full_simp_tac (del_simps (@{thm fun_upd_apply}::del_thms) (add_simps @{thms ty_repr_basic_def} ctxt))
+  | Const (@{const_name FReadMask}, _) =>
+     asm_full_simp_tac (del_simps del_thms (add_simps @{thms lift_fun_bpl_def ty_repr_basic_def} ctxt)) THEN'
+     asm_full_simp_tac ctxt
+  | _ =>      
+     asm_full_simp_tac (del_simps del_thms (add_simps @{thms lift_fun_bpl_def ty_repr_basic_def} ctxt))   
+
+fun axiom_tac ctxt fun_interp_inst_def_thm lookup_const_thms del_thms =
+  let val axiom_tac_data : axiom_tac_data = { 
+     lookup_const_tac = asm_full_simp_tac (del_simps del_thms (add_simps (@{thm lookup_full_ext_env_same} :: lookup_const_thms) ctxt)),
+     finterp_eval_tac = finterp_eval_concrete_tac del_thms,
+     fun_interp_inst_def_thm = fun_interp_inst_def_thm
+  }
+  in (fn i => fn st => axiom_aux_tac ctxt lookup_const_thms del_thms axiom_tac_data i st)
+  end
 
 \<close>
 
