ViperBoogieTranslationInterface.thy
@@ -197,7 +197,9 @@ fun fun_repr_concrete :: fun_repr_bpl
   | "fun_repr_concrete FGoodState = ''state''"
   | "fun_repr_concrete FGoodMask = ''GoodMask''"
   | "fun_repr_concrete FHasPerm = ''HasDirectPerm''"
-  | "fun_repr_concrete FIdenticalOnKnownLocs = ''IdenticalOnKnownLocations''"  
+  | "fun_repr_concrete FIdenticalOnKnownLocs = ''IdenticalOnKnownLocations''" 
+  | "fun_repr_concrete FIsPredicateField = ''IsPredicateField''"
+  | "fun_repr_concrete FIsWandField = ''IsWandField''"
 
 lemma fun_repr_concrete_inj: "inj fun_repr_concrete"
   unfolding inj_def
